[C$] Add a simpler dedicated implementation environment.
For the reasons explained in the added documentation.

books/kestrel/c/syntax/implementation-environments.lisp
@@ -28,64 +28,137 @@
   :long
   (xdoc::topstring
    (xdoc::p
-    "Our "
-    (xdoc::seetopic "c::language"
-                    "formalization of C")
-    " includes a notion of "
+    "These are similar to the "
     (xdoc::seetopic "c::implementation-environments"
                     "implementation environments")
-    ", which we also need to use for our C syntax for tools,
-     specifically for certain tools that operate on it.
-     Currently the C syntax for tools only depends on
-     some but not all aspects of implementation environments,
-     namely the applicable inputs of @(tsee input-files).
-     Here we provide a simplified constructor of implementation environments
-     that only takes some of the parameters as choices,
-     and hardwired the rest."))
+    " that are part of our C language formalization,
+     but they are simpler and meant for efficient execution.
+     The implementation environments in the language formalization
+     are richer, and meant for specification;
+     in particular, in the future they may include data
+     that may be inefficient to construct in execution.")
+   (xdoc::p
+    "We provide a mapping from these simplified implementation environments
+     to the more complex ones in the language formalization.
+     We also prove that
+     the operations on implementation environments defined here
+     are consistent with
+     the corresponding operations in the language formalization,
+     according to the aforementioned mapping."))
   :order-subtopics t
   :default-parent t)
 
 ;;;;;;;;;;;;;;;;;;;;;;;;;;;;;;;;;;;;;;;;;;;;;;;;;;;;;;;;;;;;;;;;;;;;;;;;;;;;;;;;
 
-(define ienv-simple ((short-bytes posp)
-                     (int-bytes posp)
-                     (long-bytes posp)
-                     (llong-bytes posp)
-                     (plain-chars-signed booleanp)
-                     (gcc booleanp))
-  :guard (and (>= short-bytes 2)
-              (>= int-bytes 2)
-              (>= long-bytes 4)
-              (>= llong-bytes 8)
-              (<= short-bytes int-bytes)
-              (<= int-bytes long-bytes)
-              (<= long-bytes llong-bytes))
-  :returns (ienv ienvp)
-  :short "Simplified constructor of implementation environments."
+(fty::defprod ienv
+  :short "Fixtype of implementation environments."
   :long
   (xdoc::topstring
    (xdoc::p
-    "As explained in @(see implementation-environments),
-     this only depends on the applicable inputs of @(tsee input-files):
-     see that documentation.")
+    "We assume that bytes are 8 bits,
+     that signed integers use two's complement,
+     and that there are no padding bits
+     or trap representations.
+     Therefore, the characteristics of the integer types
+     are defined by four numbers,
+     i.e. the numbers of bytes of (signed and unsigned)
+     @('short'), @('int'), @('long'), and @('long long');
+     constraints on those number are derived from
+     [C17:5.2.4.2.1] (for the minima)
+     and [C17:6.2.5/8] (for the increasing sizes).")
    (xdoc::p
-    "We set the rest of the implementation environment parameters as follows:")
-   (xdoc::ul
-    (xdoc::li
-     "Characters (i.e. bytes) are 8 bits.")
-    (xdoc::li
-     "Signed integers are two's complement.")
-    (xdoc::li
-     "There are no padding bits.")
-    (xdoc::li
-     "There are no trap representations.")))
-  (b* ((uchar-format (c::uchar-format-8))
+    "We also need a flag saying whether the plain @('char') type
+     has the same range as @('signed char') or not [C17:6.2.5/15].
+     If the flag is false, it has the same range as @('unsigned char').")
+   (xdoc::p
+    "We also need a flag saying whether GCC extensions are enabled or not.
+     This could eventually evolve into a rich set of C versions,
+     similar to the options supported by compilers like GCC."))
+  ((short-bytes pos
+                :reqfix (if (and (<= short-bytes int-bytes)
+                                 (<= int-bytes long-bytes)
+                                 (<= long-bytes llong-bytes)
+                                 (<= 2 short-bytes)
+                                 (<= 2 int-bytes)
+                                 (<= 4 long-bytes)
+                                 (<= 8 llong-bytes))
+                            short-bytes
+                          2))
+   (int-bytes pos
+              :reqfix (if (and (<= short-bytes int-bytes)
+                               (<= int-bytes long-bytes)
+                               (<= long-bytes llong-bytes)
+                               (<= 2 short-bytes)
+                               (<= 2 int-bytes)
+                               (<= 4 long-bytes)
+                               (<= 8 llong-bytes))
+                          int-bytes
+                        2))
+   (long-bytes pos
+               :reqfix (if (and (<= short-bytes int-bytes)
+                                (<= int-bytes long-bytes)
+                                (<= long-bytes llong-bytes)
+                                (<= 2 short-bytes)
+                                (<= 2 int-bytes)
+                                (<= 4 long-bytes)
+                                (<= 8 llong-bytes))
+                           long-bytes
+                         4))
+   (llong-bytes pos
+                :reqfix (if (and (<= short-bytes int-bytes)
+                                 (<= int-bytes long-bytes)
+                                 (<= long-bytes llong-bytes)
+                                 (<= 2 short-bytes)
+                                 (<= 2 int-bytes)
+                                 (<= 4 long-bytes)
+                                 (<= 8 llong-bytes))
+                            llong-bytes
+                          8))
+   (plain-char-signedp bool)
+   (gcc bool))
+  :require (and (<= short-bytes int-bytes)
+                (<= int-bytes long-bytes)
+                (<= long-bytes llong-bytes)
+                (<= 2 short-bytes)
+                (<= 2 int-bytes)
+                (<= 4 long-bytes)
+                (<= 8 llong-bytes))
+  :pred ienvp)
+
+;;;;;;;;;;;;;;;;;;;;;;;;;;;;;;;;;;;;;;;;
+
+(define ldm-ienv ((ienv ienvp))
+  :returns (ienv1 c::ienvp)
+  :short "Map an implementation environment of type @(tsee ienv)
+          to one in the language formalization of type @(tsee c::ienv)."
+  :long
+  (xdoc::topstring
+   (xdoc::p
+    "The @('ldm') part of this function's name
+     is related to the one used for the functions in @(tsee langdef-mapping),
+     since we are mapping from the C syntax for tools
+     to the formal language definition.")
+   (xdoc::p
+    "Given our assumptions (stated in @(tsee ienv))
+     that bytes are 8 bits,
+     that signed integers are two's complement,
+     and that there are no padding bits and no trap representations,
+     this mapping could still be defined in different ways,
+     based on the exact choice of bit layouts,
+     which is captured in @(tsee c::ienv) but not in @(tsee ienv).
+     We pick a simple layout, already defined in the language formalization,
+     consisting of increasing bit values,
+     ended by the sign bit for signed integers.
+     The exact choice of bit layout does not matter,
+     since the main purpose of the mapping is to exhibit a correspondence."))
+  (b* (((ienv ienv) ienv)
+       (uchar-format (c::uchar-format-8))
        (schar-format (c::schar-format-8tcnt))
-       (char-format (c::char-format plain-chars-signed))
-       (short-format (c::integer-format-inc-sign-tcnpnt (* 8 short-bytes)))
-       (int-format (c::integer-format-inc-sign-tcnpnt (* 8 int-bytes)))
-       (long-format (c::integer-format-inc-sign-tcnpnt (* 8 long-bytes)))
-       (llong-format (c::integer-format-inc-sign-tcnpnt (* 8 llong-bytes)))
+       (char-format (c::char-format ienv.plain-char-signedp))
+       (short-format (c::integer-format-inc-sign-tcnpnt (* 8 ienv.short-bytes)))
+       (int-format (c::integer-format-inc-sign-tcnpnt (* 8 ienv.int-bytes)))
+       (long-format (c::integer-format-inc-sign-tcnpnt (* 8 ienv.long-bytes)))
+       (llong-format (c::integer-format-inc-sign-tcnpnt (* 8 ienv.llong-bytes)))
        (char+short+int+long+llong-format
         (c::char+short+int+long+llong-format uchar-format
                                              schar-format
@@ -96,16 +169,29 @@
                                              llong-format)))
     (c::make-ienv
      :char+short+int+long+llong-format char+short+int+long+llong-format
-     :gcc gcc))
-  :guard-hints
-  (("Goal"
-    :in-theory
-    (enable c::char+short+int+long+llong-format-wfp
-            c::integer-format-short-wfp-of-integer-format-inc-sign-tcnpnt
-            c::integer-format-int-wfp-of-integer-format-inc-sign-tcnpnt
-            c::integer-format-long-wfp-of-integer-format-inc-sign-tcnpnt
-            c::integer-format-llong-wfp-of-integer-format-inc-sign-tcnpnt
-            fix))))
+     :gcc ienv.gcc))
+  :guard-hints (("Goal" :in-theory (enable ldm-ienv-wfp-lemma)))
+  :hooks (:fix)
+
+  :prepwork
+  ((defruled ldm-ienv-wfp-lemma
+     (c::char+short+int+long+llong-format-wfp
+      (c::char+short+int+long+llong-format
+       '((c::size . 8))
+       '((c::signed :twos-complement) (c::trap))
+       (c::char-format (ienv->plain-char-signedp ienv))
+       (c::integer-format-inc-sign-tcnpnt (* 8 (ienv->short-bytes ienv)))
+       (c::integer-format-inc-sign-tcnpnt (* 8 (ienv->int-bytes ienv)))
+       (c::integer-format-inc-sign-tcnpnt (* 8 (ienv->long-bytes ienv)))
+       (c::integer-format-inc-sign-tcnpnt (* 8 (ienv->llong-bytes ienv)))))
+     :use (:instance ienv-requirements (x ienv))
+     :enable (c::char+short+int+long+llong-format-wfp
+              c::integer-format-short-wfp-of-integer-format-inc-sign-tcnpnt
+              c::integer-format-int-wfp-of-integer-format-inc-sign-tcnpnt
+              c::integer-format-long-wfp-of-integer-format-inc-sign-tcnpnt
+              c::integer-format-llong-wfp-of-integer-format-inc-sign-tcnpnt
+              fix)
+     :disable ienv-requirements)))
 
 ;;;;;;;;;;;;;;;;;;;;;;;;;;;;;;;;;;;;;;;;;;;;;;;;;;;;;;;;;;;;;;;;;;;;;;;;;;;;;;;;
 
@@ -118,4 +204,581 @@
      but we set all the byte sizes to their minima,
      and the plain @('char') flag to @('nil') (i.e. unsigned);
      we also disable GCC extensions."))
-  (ienv-simple 2 2 4 8 nil nil))
+  (make-ienv :short-bytes 2
+             :int-bytes 2
+             :long-bytes 4
+             :llong-bytes 8
+             :plain-char-signedp nil
+             :gcc nil))
+
+;;;;;;;;;;;;;;;;;;;;;;;;;;;;;;;;;;;;;;;;;;;;;;;;;;;;;;;;;;;;;;;;;;;;;;;;;;;;;;;;
+
+(define ienv->uchar-max ((ienv ienvp))
+  :returns (max posp)
+  :short "The ACL2 integer value of @('UCHAR_MAX') [C17:5.2.4.2.1/1]."
+  :long
+  (xdoc::topstring
+   (xdoc::p
+    "Although this currently does not depend on the implementation environment,
+     we make that an input to this function for uniformity and extensibility."))
+  (declare (ignore ienv))
+  255
+  :hooks (:fix)
+  :type-prescription (and (posp (ienv->uchar-max ienv))
+                          (> (ienv->uchar-max ienv) 1))
+
+  ///
+
+  (defruled ienv->uchar-max-correct
+    (equal (ienv->uchar-max ienv)
+           (c::ienv->uchar-max (ldm-ienv ienv)))
+    :enable (ldm-ienv
+             c::ienv->uchar-max)))
+
+;;;;;;;;;;;;;;;;;;;;;;;;;;;;;;;;;;;;;;;;
+
+(define ienv->schar-max ((ienv ienvp))
+  :returns (max posp)
+  :short "The ACL2 integer value of @('SCHAR_MAX') [C17:5.2.4.2.1/1]."
+  :long
+  (xdoc::topstring
+   (xdoc::p
+    "Although this currently does not depend on the implementation environment,
+     we make that an input to this function for uniformity and extensibility."))
+  (declare (ignore ienv))
+  127
+  :hooks (:fix)
+  :type-prescription (and (posp (ienv->schar-max ienv))
+                          (> (ienv->schar-max ienv) 1))
+
+  ///
+
+  (defruled ienv->schar-max-correct
+    (equal (ienv->schar-max ienv)
+           (c::ienv->schar-max (ldm-ienv ienv)))
+    :enable (ldm-ienv
+             c::ienv->schar-max)))
+
+;;;;;;;;;;;;;;;;;;;;;;;;;;;;;;;;;;;;;;;;
+
+(define ienv->schar-min ((ienv ienvp))
+  :returns (min integerp)
+  :short "The ACL2 integer value of @('SCHAR_MIN') [C17:5.2.4.2.1/1]."
+  :long
+  (xdoc::topstring
+   (xdoc::p
+    "Although this currently does not depend on the implementation environment,
+     we make that an input to this function for uniformity and extensibility."))
+  (declare (ignore ienv))
+  -128
+  :hooks (:fix)
+  :type-prescription (integerp (ienv->schar-min ienv))
+
+  ///
+
+  (defruled ienv->schar-min-correct
+    (equal (ienv->schar-min ienv)
+           (c::ienv->schar-min (ldm-ienv ienv)))
+    :enable (ldm-ienv
+             c::ienv->schar-min)))
+
+;;;;;;;;;;;;;;;;;;;;;;;;;;;;;;;;;;;;;;;;
+
+(define ienv->char-max ((ienv ienvp))
+  :returns (max posp)
+  :short "The ACL2 integer value of @('CHAR_MAX') [C17:5.2.4.2.1/1]."
+  (if (ienv->plain-char-signedp ienv)
+      127
+    255)
+  :hooks (:fix)
+  :type-prescription (and (posp (ienv->char-max ienv))
+                          (> (ienv->char-max ienv) 1))
+
+  ///
+
+  (defruled ienv->char-max-correct
+    (equal (ienv->char-max ienv)
+           (c::ienv->char-max (ldm-ienv ienv)))
+    :enable (ldm-ienv
+             c::ienv->char-max
+             ldm-ienv-wfp-lemma)))
+
+;;;;;;;;;;;;;;;;;;;;;;;;;;;;;;;;;;;;;;;;
+
+(define ienv->char-min ((ienv ienvp))
+  :returns (min integerp)
+  :short "The ACL2 integer value of @('CHAR_MAX') [C17:5.2.4.2.1/1]."
+  (if (ienv->plain-char-signedp ienv)
+      -128
+    0)
+  :hooks (:fix)
+  :type-prescription (integerp (ienv->char-min ienv))
+
+  ///
+
+  (defruled ienv->char-min-correct
+    (equal (ienv->char-min ienv)
+           (c::ienv->char-min (ldm-ienv ienv)))
+    :enable (ldm-ienv
+             c::ienv->char-min
+             ldm-ienv-wfp-lemma)))
+
+;;;;;;;;;;;;;;;;;;;;;;;;;;;;;;;;;;;;;;;;
+
+(define ienv->ushort-max ((ienv ienvp))
+  :returns (max posp)
+  :short "The ACL2 integer value of @('USHRT_MAX') [C17:5.2.4.2.1]."
+  (1- (expt 2 (* 8 (ienv->short-bytes ienv))))
+  :hooks (:fix)
+
+  ///
+
+  (defret ienv->ushort-max-type-prescription
+    (and (posp max)
+         (> max 1))
+    :rule-classes :type-prescription)
+
+  (defruled ienv->ushort-max-correct
+    (equal (ienv->ushort-max ienv)
+           (c::ienv->ushort-max (ldm-ienv ienv)))
+    :enable (ldm-ienv
+             c::ienv->ushort-max
+             c::integer-format->unsigned-max-of-integer-format-inc-sign-tcnpnt
+             ldm-ienv-wfp-lemma)))
+
+;;;;;;;;;;;;;;;;;;;;;;;;;;;;;;;;;;;;;;;;
+
+(define ienv->sshort-max ((ienv ienvp))
+  :returns (max posp)
+  :short "The ACL2 integer value of @('SHRT_MAX') [C17:5.2.4.2.1]."
+  (1- (expt 2 (1- (* 8 (ienv->short-bytes ienv)))))
+  :hooks (:fix)
+
+  ///
+
+  (defret ienv->sshort-max-type-prescription
+    (and (posp max)
+         (> max 1))
+    :rule-classes :type-prescription)
+
+  (defruled ienv->sshort-max-correct
+    (equal (ienv->sshort-max ienv)
+           (c::ienv->sshort-max (ldm-ienv ienv)))
+    :enable (ldm-ienv
+             c::ienv->sshort-max
+             c::integer-format->signed-max-of-integer-format-inc-sign-tcnpnt
+             ldm-ienv-wfp-lemma)))
+
+;;;;;;;;;;;;;;;;;;;;;;;;;;;;;;;;;;;;;;;;
+
+(define ienv->sshort-min ((ienv ienvp))
+  :returns (min integerp :rule-classes (:rewrite :type-prescription))
+  :short "The ACL2 integer value of @('SHRT_MIN') [C17:5.2.4.2.1]."
+  (- (expt 2 (1- (* 8 (ienv->short-bytes ienv)))))
+  :hooks (:fix)
+
+  ///
+
+  (defruled ienv->sshort-min-correct
+    (equal (ienv->sshort-min ienv)
+           (c::ienv->sshort-min (ldm-ienv ienv)))
+    :enable (ldm-ienv
+             c::ienv->sshort-min
+             c::integer-format->signed-min-of-integer-format-inc-sign-tcnpnt
+             ldm-ienv-wfp-lemma)))
+
+;;;;;;;;;;;;;;;;;;;;;;;;;;;;;;;;;;;;;;;;
+
+(define ienv->uint-max ((ienv ienvp))
+  :returns (max posp)
+  :short "The ACL2 integer value of @('UINT_MAX') [C17:5.2.4.2.1]."
+  (1- (expt 2 (* 8 (ienv->int-bytes ienv))))
+  :hooks (:fix)
+
+  ///
+
+  (defret ienv->uint-max-type-prescription
+    (and (posp max)
+         (> max 1))
+    :rule-classes :type-prescription)
+
+  (defruled ienv->uint-max-correct
+    (equal (ienv->uint-max ienv)
+           (c::ienv->uint-max (ldm-ienv ienv)))
+    :enable (ldm-ienv
+             c::ienv->uint-max
+             c::integer-format->unsigned-max-of-integer-format-inc-sign-tcnpnt
+             ldm-ienv-wfp-lemma)))
+
+;;;;;;;;;;;;;;;;;;;;;;;;;;;;;;;;;;;;;;;;
+
+(define ienv->sint-max ((ienv ienvp))
+  :returns (max posp)
+  :short "The ACL2 integer value of @('INT_MAX') [C17:5.2.4.2.1]."
+  (1- (expt 2 (1- (* 8 (ienv->int-bytes ienv)))))
+  :hooks (:fix)
+
+  ///
+
+  (defret ienv->sint-max-type-prescription
+    (and (posp max)
+         (> max 1))
+    :rule-classes :type-prescription)
+
+  (defruled ienv->sint-max-correct
+    (equal (ienv->sint-max ienv)
+           (c::ienv->sint-max (ldm-ienv ienv)))
+    :enable (ldm-ienv
+             c::ienv->sint-max
+             c::integer-format->signed-max-of-integer-format-inc-sign-tcnpnt
+             ldm-ienv-wfp-lemma)))
+
+;;;;;;;;;;;;;;;;;;;;;;;;;;;;;;;;;;;;;;;;
+
+(define ienv->sint-min ((ienv ienvp))
+  :returns (min integerp :rule-classes (:rewrite :type-prescription))
+  :short "The ACL2 integer value of @('INT_MIN') [C17:5.2.4.2.1]."
+  (- (expt 2 (1- (* 8 (ienv->int-bytes ienv)))))
+  :hooks (:fix)
+
+  ///
+
+  (defruled ienv->sint-min-correct
+    (equal (ienv->sint-min ienv)
+           (c::ienv->sint-min (ldm-ienv ienv)))
+    :enable (ldm-ienv
+             c::ienv->sint-min
+             c::integer-format->signed-min-of-integer-format-inc-sign-tcnpnt
+             ldm-ienv-wfp-lemma)))
+
+;;;;;;;;;;;;;;;;;;;;;;;;;;;;;;;;;;;;;;;;
+
+(define ienv->ulong-max ((ienv ienvp))
+  :returns (max posp)
+  :short "The ACL2 integer value of @('ULONG_MAX') [C17:5.2.4.2.1]."
+  (1- (expt 2 (* 8 (ienv->long-bytes ienv))))
+  :hooks (:fix)
+
+  ///
+
+  (defret ienv->ulong-max-type-prescription
+    (and (posp max)
+         (> max 1))
+    :rule-classes :type-prescription)
+
+  (defruled ienv->ulong-max-correct
+    (equal (ienv->ulong-max ienv)
+           (c::ienv->ulong-max (ldm-ienv ienv)))
+    :enable (ldm-ienv
+             c::ienv->ulong-max
+             c::integer-format->unsigned-max-of-integer-format-inc-sign-tcnpnt
+             ldm-ienv-wfp-lemma)))
+
+;;;;;;;;;;;;;;;;;;;;;;;;;;;;;;;;;;;;;;;;
+
+(define ienv->slong-max ((ienv ienvp))
+  :returns (max posp)
+  :short "The ACL2 integer value of @('LONG_MAX') [C17:5.2.4.2.1]."
+  (1- (expt 2 (1- (* 8 (ienv->long-bytes ienv)))))
+  :hooks (:fix)
+
+  ///
+
+  (defret ienv->slong-max-type-prescription
+    (and (posp max)
+         (> max 1))
+    :rule-classes :type-prescription)
+
+  (defruled ienv->slong-max-correct
+    (equal (ienv->slong-max ienv)
+           (c::ienv->slong-max (ldm-ienv ienv)))
+    :enable (ldm-ienv
+             c::ienv->slong-max
+             c::integer-format->signed-max-of-integer-format-inc-sign-tcnpnt
+             ldm-ienv-wfp-lemma)))
+
+;;;;;;;;;;;;;;;;;;;;;;;;;;;;;;;;;;;;;;;;
+
+(define ienv->slong-min ((ienv ienvp))
+  :returns (min integerp :rule-classes (:rewrite :type-prescription))
+  :short "The ACL2 integer value of @('LONG_MIN') [C17:5.2.4.2.1]."
+  (- (expt 2 (1- (* 8 (ienv->long-bytes ienv)))))
+  :hooks (:fix)
+
+  ///
+
+  (defruled ienv->slong-min-correct
+    (equal (ienv->slong-min ienv)
+           (c::ienv->slong-min (ldm-ienv ienv)))
+    :enable (ldm-ienv
+             c::ienv->slong-min
+             c::integer-format->signed-min-of-integer-format-inc-sign-tcnpnt
+             ldm-ienv-wfp-lemma)))
+
+;;;;;;;;;;;;;;;;;;;;;;;;;;;;;;;;;;;;;;;;
+
+(define ienv->ullong-max ((ienv ienvp))
+  :returns (max posp)
+  :short "The ACL2 integer value of @('ULLONG_MAX') [C17:5.2.4.2.1]."
+  (1- (expt 2 (* 8 (ienv->llong-bytes ienv))))
+  :hooks (:fix)
+
+  ///
+
+  (defret ienv->ullong-max-type-prescription
+    (and (posp max)
+         (> max 1))
+    :rule-classes :type-prescription)
+
+  (defruled ienv->ullong-max-correct
+    (equal (ienv->ullong-max ienv)
+           (c::ienv->ullong-max (ldm-ienv ienv)))
+    :enable (ldm-ienv
+             c::ienv->ullong-max
+             c::integer-format->unsigned-max-of-integer-format-inc-sign-tcnpnt
+             ldm-ienv-wfp-lemma)))
+
+;;;;;;;;;;;;;;;;;;;;;;;;;;;;;;;;;;;;;;;;
+
+(define ienv->sllong-max ((ienv ienvp))
+  :returns (max posp)
+  :short "The ACL2 integer value of @('LLONG_MAX') [C17:5.2.4.2.1]."
+  (1- (expt 2 (1- (* 8 (ienv->llong-bytes ienv)))))
+  :hooks (:fix)
+
+  ///
+
+  (defret ienv->sllong-max-type-prescription
+    (and (posp max)
+         (> max 1))
+    :rule-classes :type-prescription)
+
+  (defruled ienv->sllong-max-correct
+    (equal (ienv->sllong-max ienv)
+           (c::ienv->sllong-max (ldm-ienv ienv)))
+    :enable (ldm-ienv
+             c::ienv->sllong-max
+             c::integer-format->signed-max-of-integer-format-inc-sign-tcnpnt
+             ldm-ienv-wfp-lemma)))
+
+;;;;;;;;;;;;;;;;;;;;;;;;;;;;;;;;;;;;;;;;
+
+(define ienv->sllong-min ((ienv ienvp))
+  :returns (min integerp :rule-classes (:rewrite :type-prescription))
+  :short "The ACL2 integer value of @('LLONG_MIN') [C17:5.2.4.2.1]."
+  (- (expt 2 (1- (* 8 (ienv->llong-bytes ienv)))))
+  :hooks (:fix)
+
+  ///
+
+  (defruled ienv->sllong-min-correct
+    (equal (ienv->sllong-min ienv)
+           (c::ienv->sllong-min (ldm-ienv ienv)))
+    :enable (ldm-ienv
+             c::ienv->sllong-min
+             c::integer-format->signed-min-of-integer-format-inc-sign-tcnpnt
+             ldm-ienv-wfp-lemma)))
+
+;;;;;;;;;;;;;;;;;;;;;;;;;;;;;;;;;;;;;;;;;;;;;;;;;;;;;;;;;;;;;;;;;;;;;;;;;;;;;;;;
+
+(define ienv-uchar-rangep ((val integerp) (ienv ienvp))
+  :returns (yes/no booleanp)
+  :short "Check if an ACl2 integer is
+          in the range of (i.e. representable in) type @('unsigned char')."
+  (and (<= 0 (ifix val))
+       (<= (ifix val) (ienv->uchar-max ienv)))
+  :hooks (:fix)
+
+  ///
+
+  (defruled ienv-uchar-rangep-correct
+    (equal (ienv-uchar-rangep val ienv)
+           (c::ienv-uchar-rangep val (ldm-ienv ienv)))
+    :enable (c::ienv-uchar-rangep
+             ienv->uchar-max-correct)))
+
+;;;;;;;;;;;;;;;;;;;;;;;;;;;;;;;;;;;;;;;;
+
+(define ienv-schar-rangep ((val integerp) (ienv ienvp))
+  :returns (yes/no booleanp)
+  :short "Check if an ACl2 integer is
+          in the range of (i.e. representable in) type @('signed char')."
+  (and (<= (ienv->schar-min ienv) (ifix val))
+       (<= (ifix val) (ienv->schar-max ienv)))
+  :hooks (:fix)
+
+  ///
+
+  (defruled ienv-schar-rangep-correct
+    (equal (ienv-schar-rangep val ienv)
+           (c::ienv-schar-rangep val (ldm-ienv ienv)))
+    :enable (c::ienv-schar-rangep
+             ienv->schar-max-correct
+             ienv->schar-min-correct)))
+
+;;;;;;;;;;;;;;;;;;;;;;;;;;;;;;;;;;;;;;;;
+
+(define ienv-char-rangep ((val integerp) (ienv ienvp))
+  :returns (yes/no booleanp)
+  :short "Check if an ACl2 integer is
+          in the range of (i.e. representable in) type @('char')."
+  (and (<= (ienv->char-min ienv) (ifix val))
+       (<= (ifix val) (ienv->char-max ienv)))
+  :hooks (:fix)
+
+  ///
+
+  (defruled ienv-char-rangep-correct
+    (equal (ienv-char-rangep val ienv)
+           (c::ienv-char-rangep val (ldm-ienv ienv)))
+    :enable (c::ienv-char-rangep
+             ienv->char-max-correct
+             ienv->char-min-correct)))
+
+;;;;;;;;;;;;;;;;;;;;;;;;;;;;;;;;;;;;;;;;
+
+(define ienv-ushort-rangep ((val integerp) (ienv ienvp))
+  :returns (yes/no booleanp)
+  :short "Check if an ACl2 integer is
+          in the range of (i.e. representable in) type @('unsigned short')."
+  (and (<= 0 (ifix val))
+       (<= (ifix val) (ienv->ushort-max ienv)))
+  :hooks (:fix)
+
+  ///
+
+  (defruled ienv-ushort-rangep-correct
+    (equal (ienv-ushort-rangep val ienv)
+           (c::ienv-ushort-rangep val (ldm-ienv ienv)))
+    :enable (c::ienv-ushort-rangep
+             ienv->ushort-max-correct)))
+
+;;;;;;;;;;;;;;;;;;;;;;;;;;;;;;;;;;;;;;;;
+
+(define ienv-sshort-rangep ((val integerp) (ienv ienvp))
+  :returns (yes/no booleanp)
+  :short "Check if an ACl2 integer is
+          in the range of (i.e. representable in) type @('signed short')."
+  (and (<= (ienv->sshort-min ienv) (ifix val))
+       (<= (ifix val) (ienv->sshort-max ienv)))
+  :hooks (:fix)
+
+  ///
+
+  (defruled ienv-sshort-rangep-correct
+    (equal (ienv-sshort-rangep val ienv)
+           (c::ienv-sshort-rangep val (ldm-ienv ienv)))
+    :enable (c::ienv-sshort-rangep
+             ienv->sshort-max-correct
+             ienv->sshort-min-correct)))
+
+;;;;;;;;;;;;;;;;;;;;;;;;;;;;;;;;;;;;;;;;
+
+(define ienv-uint-rangep ((val integerp) (ienv ienvp))
+  :returns (yes/no booleanp)
+  :short "Check if an ACl2 integer is
+          in the range of (i.e. representable in) type @('unsigned int')."
+  (and (<= 0 (ifix val))
+       (<= (ifix val) (ienv->uint-max ienv)))
+  :hooks (:fix)
+
+  ///
+
+  (defruled ienv-uint-rangep-correct
+    (equal (ienv-uint-rangep val ienv)
+           (c::ienv-uint-rangep val (ldm-ienv ienv)))
+    :enable (c::ienv-uint-rangep
+             ienv->uint-max-correct)))
+
+;;;;;;;;;;;;;;;;;;;;;;;;;;;;;;;;;;;;;;;;
+
+(define ienv-sint-rangep ((val integerp) (ienv ienvp))
+  :returns (yes/no booleanp)
+  :short "Check if an ACl2 integer is
+          in the range of (i.e. representable in) type @('signed int')."
+  (and (<= (ienv->sint-min ienv) (ifix val))
+       (<= (ifix val) (ienv->sint-max ienv)))
+  :hooks (:fix)
+
+  ///
+
+  (defruled ienv-sint-rangep-correct
+    (equal (ienv-sint-rangep val ienv)
+           (c::ienv-sint-rangep val (ldm-ienv ienv)))
+    :enable (c::ienv-sint-rangep
+             ienv->sint-max-correct
+             ienv->sint-min-correct)))
+
+;;;;;;;;;;;;;;;;;;;;;;;;;;;;;;;;;;;;;;;;
+
+(define ienv-ulong-rangep ((val integerp) (ienv ienvp))
+  :returns (yes/no booleanp)
+  :short "Check if an ACl2 integer is
+          in the range of (i.e. representable in) type @('unsigned long')."
+  (and (<= 0 (ifix val))
+       (<= (ifix val) (ienv->ulong-max ienv)))
+  :hooks (:fix)
+
+  ///
+
+  (defruled ienv-ulong-rangep-correct
+    (equal (ienv-ulong-rangep val ienv)
+           (c::ienv-ulong-rangep val (ldm-ienv ienv)))
+    :enable (c::ienv-ulong-rangep
+             ienv->ulong-max-correct)))
+
+;;;;;;;;;;;;;;;;;;;;;;;;;;;;;;;;;;;;;;;;
+
+(define ienv-slong-rangep ((val integerp) (ienv ienvp))
+  :returns (yes/no booleanp)
+  :short "Check if an ACl2 integer is
+          in the range of (i.e. representable in) type @('signed long')."
+  (and (<= (ienv->slong-min ienv) (ifix val))
+       (<= (ifix val) (ienv->slong-max ienv)))
+  :hooks (:fix)
+
+  ///
+
+  (defruled ienv-slong-rangep-correct
+    (equal (ienv-slong-rangep val ienv)
+           (c::ienv-slong-rangep val (ldm-ienv ienv)))
+    :enable (c::ienv-slong-rangep
+             ienv->slong-max-correct
+             ienv->slong-min-correct)))
+
+;;;;;;;;;;;;;;;;;;;;;;;;;;;;;;;;;;;;;;;;
+
+(define ienv-ullong-rangep ((val integerp) (ienv ienvp))
+  :returns (yes/no booleanp)
+  :short "Check if an ACl2 integer is
+          in the range of (i.e. representable in) type @('unsigned long long')."
+  (and (<= 0 (ifix val))
+       (<= (ifix val) (ienv->ullong-max ienv)))
+  :hooks (:fix)
+
+  ///
+
+  (defruled ienv-ullong-rangep-correct
+    (equal (ienv-ullong-rangep val ienv)
+           (c::ienv-ullong-rangep val (ldm-ienv ienv)))
+    :enable (c::ienv-ullong-rangep
+             ienv->ullong-max-correct)))
+
+;;;;;;;;;;;;;;;;;;;;;;;;;;;;;;;;;;;;;;;;
+
+(define ienv-sllong-rangep ((val integerp) (ienv ienvp))
+  :returns (yes/no booleanp)
+  :short "Check if an ACl2 integer is
+          in the range of (i.e. representable in) type @('signed long long')."
+  (and (<= (ienv->sllong-min ienv) (ifix val))
+       (<= (ifix val) (ienv->sllong-max ienv)))
+  :hooks (:fix)
+
+  ///
+
+  (defruled ienv-sllong-rangep-correct
+    (equal (ienv-sllong-rangep val ienv)
+           (c::ienv-sllong-rangep val (ldm-ienv ienv)))
+    :enable (c::ienv-sllong-rangep
+             ienv->sllong-max-correct
+             ienv->sllong-min-correct)))
